deps/coq-poulet4/lib/Step.v
@@ -2,7 +2,7 @@ Require Import Coq.Lists.List.
 Require Import Coq.Strings.String.
 Require Import Syntax.
 Require Import Eval.
-Require Import Environment.
+Require Import Environment.Environment.
 Require Import Monads.Monad.
 Require Import Monads.State.
 
